src/inductive/inductive_graph_measure.v
@@ -1,0 +1,164 @@
+
+
+Require Import Recdef.
+Require Import Lia.
+
+Require Import Coq.Arith.Arith.
+Require Import Coq.Arith.Wf_nat.
+Require Import Coq.Lists.List.
+Require Import Coq.Wellfounded.Wellfounded.
+Require Import Coq.Wellfounded.Lexicographic_Product.
+Require Import Coq.Structures.OrderedType.
+Require Import Coq.Structures.OrderedTypeEx.
+
+Import ListNotations.
+Require Import Coq.Wellfounded.Inverse_Image.
+Require Import Coq.Relations.Relation_Operators.
+
+Require Import GraphVerification.src.util.util.
+Require Import GraphVerification.src.util.NatMap.
+Require Import GraphVerification.src.inductive.inductive_graph.
+
+
+
+
+(* This proof is adapted from the link below. It blows my mind, that this is not in stdlib *)
+(* https://github.com/rocq-prover/stdlib/blob/master/theories/FSets/FMapFacts.v *)
+(* TODO: this kills coq, omg *)
+Lemma cardinal_Add_In:
+    forall (A : Type) (m m' : NatMap.t A) x e, NatMap.In x m -> MProps.Add x e m m' -> NatMap.cardinal m' = NatMap.cardinal m.
+  Proof.
+  assert (forall {A : Type} (k : Node) (e : A ) m, NatMap.MapsTo k e m -> MProps.Add k e (NatMap.remove k m) m) as remove_In_Add.
+  { intros. unfold MProps.Add.
+    intros.
+    rewrite MFacts.add_o.
+    destruct (MFacts.eq_dec k y).
+    - apply NatMap.find_1. rewrite <- MFacts.MapsTo_m; [exact H|assumption|reflexivity|reflexivity].
+    - rewrite MFacts.remove_neq_o by assumption. reflexivity.
+  }
+  intros.
+  assert (NatMap.Equal (NatMap.remove x m) (NatMap.remove x m')).
+  { intros y. rewrite 2!MFacts.remove_o.
+    destruct (MFacts.eq_dec x y).
+    - reflexivity.
+    - unfold MProps.Add in H0. rewrite H0.
+      rewrite MFacts.add_neq_o by assumption. reflexivity.
+  }
+  Admitted.
+  (* apply MProps.Equal_cardinal in H1.
+  rewrite 2!MProps.cardinal_fold.
+  destruct H as (e' & H).
+  rewrite MProps.fold_Add with (eqA:=eq) (m1:=NatMap.remove x m) (m2:=m) (k:=x) (e:=e');
+  try now (compute; auto).
+  2:apply NatMap.remove_1; reflexivity.
+  2:apply remove_In_Add; assumption.
+  rewrite MProps.fold_Add with (eqA:=eq) (m1:=NatMap.remove x m') (m2:=m') (k:=x) (e:=e);
+  try now (compute; auto).
+  - rewrite <- 2!MProps.cardinal_fold. congruence.
+  - apply NatMap.remove_1. reflexivity.
+  - apply remove_In_Add.
+    apply NatMap.find_2. unfold MProps.Add in H0. rewrite H0.
+    rewrite MFacts.add_eq_o; reflexivity.
+  Qed. *)
+
+
+
+Lemma _add_value_does_not_matter_for_cardinality : forall {A : Type} (node : Node) (c c' : A) (m : NatMap.t A),
+  NatMap.cardinal (NatMap.add node c m) = NatMap.cardinal (NatMap.add node c' m).
+Proof.
+  intros.
+  pose proof cardinal_Add_In.
+  apply (H _ _ _ node c).
+  - apply MFacts.add_in_iff. left. reflexivity.
+  - unfold MProps.Add. intros. rewrite MFacts.add_o. rewrite MFacts.add_o. rewrite MFacts.add_o. destruct (MProps.F.eq_dec node y).
+    + reflexivity.
+    + reflexivity.
+Qed.
+
+
+
+
+
+
+Lemma _IG_updateEntry_does_not_change_cardinality : forall {A B : Type} (node : Node) (f : Context' A B -> Context' A B) (ig : IG A B), 
+    NatMap.cardinal (_updateEntry node f ig) = NatMap.cardinal ig.
+Proof.
+  intros. unfold _updateEntry.
+
+  destruct (NatMap.find node ig) eqn:split.
+  - 
+
+  assert (NatMap.Equal ig (NatMap.add node c ig)). { 
+      apply MFacts.find_mapsto_iff in split.
+
+    apply MFacts.Equal_mapsto_iff.
+    split; intros.
+    - apply MFacts.add_mapsto_iff.
+       bdestruct (node =? k).
+      + subst. left. split.
+      -- reflexivity.
+      -- apply MFacts.find_mapsto_iff in split. apply MFacts.find_mapsto_iff in H. rewrite H in split. inversion split. reflexivity.
+      + right. split.
+      -- assumption.
+      -- assumption.
+    - apply MFacts.add_mapsto_iff in H. destruct H.
+      + destruct H. subst. assumption.
+      + destruct H. assumption.
+  }
+  rewrite H at 2.
+  apply _add_value_does_not_matter_for_cardinality.
+  - reflexivity.
+
+Qed.
+
+
+
+Lemma _IG_updAdj_does_not_change_cardinality : forall {A B : Type} (adj : Adj B) (f : B -> Context' A B -> Context' A B) (ig : IG A B), 
+    NatMap.cardinal (_updAdj adj f ig) = NatMap.cardinal ig.
+Proof.
+  intros.
+  unfold _updAdj.
+  induction adj.
+  - simpl. reflexivity.
+  - simpl. rewrite <- IHadj.
+    pose proof (@_IG_updateEntry_does_not_change_cardinality A B).
+    destruct a.
+    rewrite H. reflexivity.
+Qed.
+
+
+Lemma _map_find_some_remove_lowers_cardinality : forall {A : Type} (key : Node) (map : NatMap.t A),
+  (exists x, NatMap.find key map = Some x) -> (S (NatMap.cardinal (NatMap.remove key map)) = NatMap.cardinal map).
+Proof.
+  
+  intros.
+  pose proof MProps.cardinal_2.
+  destruct H eqn:hu.
+  assert (~ NatMap.In key (NatMap.remove key map)). {
+    unfold not. intros.
+    apply MFacts.remove_in_iff in H1.
+    destruct H1.
+    destruct H1.
+    reflexivity.
+
+  }
+  apply (H0 _ _ map _ x) in H1.
+  - rewrite <- H1. reflexivity.
+  - unfold MProps.Add. 
+  
+  
+  
+  unfold MProps.Add. intros. bdestruct (y =? key).
+  + rewrite H2. rewrite e. assert (key = key). {
+    reflexivity.
+  }  pose proof MFacts.add_eq_o. apply (H4 A (NatMap.remove (elt:=A) key map) _ _ x) in H3. rewrite H3. reflexivity.
+  + pose proof MFacts.add_neq_o. assert (key <> y). {lia. } apply (H3 A (NatMap.remove (elt:=A) key map) _ _ x) in H4. rewrite H4.
+    pose proof MFacts.remove_neq_o. assert (key <> y). {lia. }  apply (H5 A map _ _) in H6. rewrite H6. reflexivity.
+  
+Defined.
+
+
+
+
+
+
